new-ocaml-compiler/theories/Correctness.v
@@ -11,8 +11,9 @@
 
 From Stdlib Require Import ZArith Strings.String PeanoNat.
 From Stdlib Require Import List. Import ListNotations.
-From OCamlInterp Require Import Value Bytecode Machine Interp Syntax
-                                Observable SourceInterp Compile.
+From OCamlInterp.Trusted Require Import Value Bytecode Machine Interp.
+From OCamlInterp.SemiTrusted Require Import Syntax Observable.
+From OCamlInterp.Untrusted Require Import SourceInterp Compile.
 Open Scope Z_scope.
 
 (* === Behavior extraction from bytecode interpreter === *)
