new-ocaml-compiler/theories/Trusted/Main.v
@@ -6,7 +6,7 @@ From Stdlib Require Import ZArith PeanoNat.
 From Stdlib Require Import List. Import ListNotations.
 From Stdlib Require Import Strings.String.
 From Stdlib Require Import Ascii.
-From OCamlInterp Require Import Value Bytecode Machine Interp Loader IO.
+From OCamlInterp.Trusted Require Import Value Bytecode Machine Interp Loader IO.
 Open Scope Z_scope.
 Open Scope bool_scope.
 
